\documentclass[11pt,letterpaper]{article}
\usepackage{amssymb}
\usepackage[fleqn]{amsmath}
\usepackage{bbm}
\usepackage{fullpage}

\begin{document}

Zackery Field

ID: 23031734

CS 70, Summer 2013

Homework 1 

Problem 3 (9 Points)
\bigskip

\begin{enumerate}
\item[3a.] [3 points]

Theorem:
$ \neg \forall x \exists y (P(x) \Rightarrow \neg Q(x,y)) \equiv \exists x \forall y (P(x) \wedge Q(x,y) )$

Proof:

\begin{eqnarray}
\neg \forall x \exists y (P(x) \Rightarrow \neg Q(x,y)) \equiv \exists x \forall y (P(x) \wedge Q(x,y) ) \\
\exists x \neg \exists y (P(x) \Rightarrow \neg Q(x,y)) \equiv \exists x \forall y (P(x) \wedge Q(x,y) ) \\
\exists x \forall y \neg (P(x) \Rightarrow \neg Q(x,y)) \equiv \exists x \forall y (P(x) \wedge Q(x,y) ) \\
\neg (P(x) \Rightarrow \neg Q(x,y)) \equiv (P(x) \wedge Q(x,y) )
\end{eqnarray}

Proof by Truth Table: 

\begin{tabular} {1 | c |c | c || c}
	\hline
	P & Q & $ \neg (P(x) \Rightarrow \neg Q(x,y))$ & $(P(x) \wedge Q(x,y) )$ \\ \hline
	T & T & T & T \\
	T & F & F & F \\
	F & T & F & F \\
	F & F & F & F \\
	\hline
\end{tabular}

After removing the equivalent quantifiers, the truth table demonstrates that the equivalence holds.

\bigskip
\item[3b.][3 points]

Theorem:
$ \forall x \exists y (P(x) \Rightarrow Q(x,y) ) \equiv \forall (P(x) \Rightarrow (\exists Q(x,y))$

Proof:

\begin{eqnarray}
\forall x \exists y (P(x) \Rightarrow Q(x,y) ) \equiv \forall x (P(x) \Rightarrow (\exists Q(x,y)) \\
\forall x \exists y (\neg P(x) \vee Q(x,y) ) \equiv \forall x (\neg P(x) \vee (\exists Q(x,y)) \\
\forall x ( (\exists y \neg P(x)) \vee (\exists y (x,y)) ) \equiv \forall x (\neg P(x) \vee (\exists Q(x,y)) \\
\forall x ( \neg P(x) \vee (\exists y (x,y)) ) \equiv \forall x (\neg P(x) \vee (\exists Q(x,y))
\end{eqnarray}

Distributing the quantifiers across disjunction statements, and removing the $\exists y$ from $P(x)$ demonstrates that the equivalence holds.


\bigskip
\item[3c.] [3 points]

Theorem:
$ \forall x \exists y (Q(x,y) \Rightarrow P(x)) \equiv \forall x ((\exists y Q(x,y)) \Rightarrow P(x)) $

Proof:
\begin{eqnarray}
\forall x \exists y (Q(x,y) \Rightarrow P(x)) \equiv \forall x ((\exists y Q(x,y)) \Rightarrow P(x)) \\
\forall x \exists y (\neg Q(x,y) \vee P(x)) \equiv \forall x (\neg (\exists y Q(x,y)) \vee P(x))  \\
\forall x (\exists y  \neg Q(x,y) \vee  \exists y P(x)) \equiv \forall x (\neg (\exists y Q(x,y)) \vee P(x))  \\
\forall x (\exists y  \neg Q(x,y) \vee  P(x)) \neq \forall x (\forall y  \neg Q(x,y) \vee P(x))
\end{eqnarray}

The equivalence does not hold due to the difference in quantifier associated with Q(x,y).

\end{enumerate}

\end{document}
